WIP: PDDL to temporal planning

Ground_PDDL_Exec_Imp/PDDL_TP_Reduction.thy
@@ -3,27 +3,599 @@ theory PDDL_TP_Reduction
     "TP_NTA_Reduction.TP_NTA_Reduction_Model_Checking"
 begin
 
+find_theorems name: "rat*linorder"
+
+instantiation lower_bound::(linorder) linorder
+begin
+fun less_eq_lower_bound::"('a::linorder) lower_bound \<Rightarrow> ('a::linorder) lower_bound \<Rightarrow> bool" where
+"less_eq_lower_bound (lower_bound.GE x) (lower_bound.GE y) = (x \<le> y)" |
+"less_eq_lower_bound (lower_bound.GE x) (lower_bound.GT y) = (x \<le> y)" |
+"less_eq_lower_bound (lower_bound.GT x) (lower_bound.GE y) = (x < y)" |
+"less_eq_lower_bound (lower_bound.GT x) (lower_bound.GT y) = (x \<le> y)"
+
+fun less_lower_bound::"('a::linorder) lower_bound \<Rightarrow> ('a::linorder) lower_bound \<Rightarrow> bool"  where
+"less_lower_bound (lower_bound.GE x) (lower_bound.GE y) = (x < y)" |
+"less_lower_bound (lower_bound.GE x) (lower_bound.GT y) = (x \<le> y)" |
+"less_lower_bound (lower_bound.GT x) (lower_bound.GE y) = (x < y)" |
+"less_lower_bound (lower_bound.GT x) (lower_bound.GT y) = (x < y)"
+instance 
+proof 
+  fix x y::"('a::linorder) lower_bound"
+  show "(x < y) = (x \<le> y \<and> \<not>y \<le> x)" 
+    by (cases x; cases y) auto
+next
+  fix x::"('a::linorder) lower_bound"
+  show "x \<le> x" by (cases x) auto
+next 
+  fix x y z::"('a::linorder) lower_bound"
+  show "x \<le> y \<Longrightarrow> y \<le> z \<Longrightarrow> x \<le> z"
+    by (cases x; cases y; cases z) auto
+next
+  fix x y::"('a::linorder) lower_bound"
+  show "x \<le> y \<Longrightarrow> y \<le> x \<Longrightarrow> x = y"
+    by (cases x; cases y) auto
+next
+  fix x y::"('a::linorder) lower_bound"
+  show "x \<le> y \<or> y \<le> x "
+    by (cases x; cases y) auto
+qed
+end
+
+instantiation upper_bound::(linorder) linorder
+begin
+fun less_eq_upper_bound::"('a::linorder) upper_bound \<Rightarrow> ('a::linorder) upper_bound \<Rightarrow> bool" where
+"less_eq_upper_bound (upper_bound.LT x) (upper_bound.LT y) = (x \<le> y)" |
+"less_eq_upper_bound (upper_bound.LT x) (upper_bound.LE y) = (x \<le> y)" |
+"less_eq_upper_bound (upper_bound.LE x) (upper_bound.LT y) = (x < y)" |
+"less_eq_upper_bound (upper_bound.LE x) (upper_bound.LE y) = (x \<le> y)"
+
+fun less_upper_bound::"('a::linorder) upper_bound \<Rightarrow> ('a::linorder) upper_bound \<Rightarrow> bool"  where
+"less_upper_bound (upper_bound.LT x) (upper_bound.LT y) = (x < y)" |
+"less_upper_bound (upper_bound.LT x) (upper_bound.LE y) = (x \<le> y)" |
+"less_upper_bound (upper_bound.LE x) (upper_bound.LT y) = (x < y)" |
+"less_upper_bound (upper_bound.LE x) (upper_bound.LE y) = (x < y)"
+instance 
+proof 
+  fix x y::"('a::linorder) upper_bound"
+  show "(x < y) = (x \<le> y \<and> \<not>y \<le> x)" 
+    by (cases x; cases y) auto
+next
+  fix x::"('a::linorder) upper_bound"
+  show "x \<le> x" by (cases x) auto
+next 
+  fix x y z::"('a::linorder) upper_bound"
+  show "x \<le> y \<Longrightarrow> y \<le> z \<Longrightarrow> x \<le> z"
+    by (cases x; cases y; cases z) auto
+next
+  fix x y::"('a::linorder) upper_bound"
+  show "x \<le> y \<Longrightarrow> y \<le> x \<Longrightarrow> x = y"
+    by (cases x; cases y) auto
+next
+  fix x y::"('a::linorder) upper_bound"
+  show "x \<le> y \<or> y \<le> x "
+    by (cases x; cases y) auto
+qed
+end
+
+fun comp_opt_le::"('a::linorder) option \<Rightarrow> ('a::linorder) option \<Rightarrow> bool" where
+"comp_opt_le None None = True" |
+"comp_opt_le None (Some x) = False" |
+"comp_opt_le (Some x) None = True" |
+"comp_opt_le (Some x) (Some y) = (x \<le> y)" 
+
+fun comp_opt_ge::"('a::linorder) option \<Rightarrow> ('a::linorder) option \<Rightarrow> bool" where
+"comp_opt_ge None None = True" |
+"comp_opt_ge None (Some x) = False" |
+"comp_opt_ge (Some x) None = True" |
+"comp_opt_ge (Some x) (Some y) = (x \<ge> y)"
+
 context ast_problem
 begin
 
-definition "prop_spec = map pred (predicates D)"
+definition "props_spec \<equiv> map pred (predicates D)"
 
-definition "act_spec = actions D"
+definition "prop_to_name_spec \<equiv> predicate.name #> String.implode"
 
-fun to_object::"object atom Formulas.formula \<Rightarrow> predicate" where
-"to_object (Atom (predAtm x _)) = x"
+definition "actions_spec \<equiv> actions D"
 
-definition "init_spec = I"
+definition "act_to_name_spec \<equiv> ast_action_schema.name #> String.implode"
+
+
+fun to_predicate::"object atom Formulas.formula \<Rightarrow> predicate" where
+"to_predicate (Atom (predAtm x _)) = x"
+
+fun to_literals::"object atom Formulas.formula \<Rightarrow> object atom Formulas.formula list" where
+"to_literals (Atom (predAtm x as)) = [Atom (predAtm x as)]" |
+"to_literals (x \<^bold>\<and> y) = to_literals x @ to_literals y" |
+"to_literals (\<^bold>\<not>\<bottom>) = []"
+
+definition "to_predicates \<equiv> to_literals #> map to_predicate"
+
+definition init_spec::"predicate list" where
+"init_spec \<equiv>
+  init P
+  |> map to_predicate
+  |> remdups"
+
+
+(* To do: ensure that this consists of predicates only *)
+definition goal_spec::"predicate list" where
+  "goal_spec \<equiv> 
+  goal P
+  |> to_literals
+  |> map to_predicate
+  |> remdups"
+
+definition "non_ground_action \<equiv> Ground_Action (Formulas.Not Formulas.Bot) (Effect [] [])"
+
+
+fun at_start_spec::"ast_action_schema \<Rightarrow> ground_action" where
+"at_start_spec (Simple_Action_Schema n ps pre eff) = instantiate_action_schema (Simple_Action_Schema n ps pre eff) []" |
+"at_start_spec (Durative_Action_Schema n ps d cond eff) = inst_snap_action (Durative_Action_Schema n ps d cond eff) [] At_Start"
+
+fun at_end_spec::"ast_action_schema \<Rightarrow> ground_action" where
+"at_end_spec (Simple_Action_Schema n ps pre eff) = non_ground_action" |
+"at_end_spec (Durative_Action_Schema n ps d cond eff) = inst_snap_action (Durative_Action_Schema n ps d cond eff) [] At_End"
+
+fun over_all_snap::"ast_action_schema \<Rightarrow> ground_action" where
+"over_all_snap (Simple_Action_Schema n ps pre eff) = 
+  non_ground_action" |
+"over_all_snap (Durative_Action_Schema n ps d cond eff) = 
+  inst_snap_action (Durative_Action_Schema n ps d cond eff) [] Over_All"
+
+fun pre_spec::"ground_action \<Rightarrow> predicate list" where
+"pre_spec (Ground_Action form eff) = 
+  form
+  |> to_literals
+  |> map to_predicate
+  |> remdups"
+
+fun over_all_spec::"ast_action_schema \<Rightarrow> predicate list" where
+"over_all_spec x =
+  x
+  |> over_all_snap
+  |> pre_spec"
+
+fun adds_spec::"ground_action \<Rightarrow> predicate list" where
+"adds_spec (Ground_Action form eff) =
+  eff
+  |> ast_effect.adds
+  |> map to_predicate
+  |> remdups
+"
+
+fun dels_spec::"ground_action \<Rightarrow> predicate list" where
+"dels_spec (Ground_Action form eff) =
+  eff
+  |> ast_effect.dels
+  |> map to_predicate
+  |> remdups
+"
+
+fun dc_to_lb::"term duration_constraint \<Rightarrow> int lower_bound option" where
+"dc_to_lb No_Const = None" |
+"dc_to_lb (Time_Const duration_op.EQ x) = Some (lower_bound.GE (floor x))" |
+"dc_to_lb (Time_Const duration_op.GEQ x) = Some (lower_bound.GE (floor x))" |
+"dc_to_lb (Time_Const duration_op.LEQ x) = None"
+
+fun max_lb_opt::"int lower_bound option list \<Rightarrow> int lower_bound option \<Rightarrow> int lower_bound option" where
+"max_lb_opt [] l = l" |
+"max_lb_opt (x#xs) l = max_lb_opt xs (if (comp_opt_ge x l) then x else l)"
+
+fun dc_list_lower::"term duration_constraint list \<Rightarrow> int lower_bound option" where
+"dc_list_lower xs = map dc_to_lb xs |> (\<lambda>xs. max_lb_opt xs None)" 
+
+
+fun dc_to_ub::"term duration_constraint \<Rightarrow> int upper_bound option" where
+"dc_to_ub No_Const = None" |
+"dc_to_ub (Time_Const duration_op.EQ x) = Some (upper_bound.LE (floor x))" |
+"dc_to_ub (Time_Const duration_op.GEQ x) = None" |
+"dc_to_ub (Time_Const duration_op.LEQ x) = Some (upper_bound.LE (floor x))"
+
+fun min_ub_opt::"int upper_bound option list \<Rightarrow> int upper_bound option \<Rightarrow> int upper_bound option" where
+"min_ub_opt [] u = u" |
+"min_ub_opt (x#xs) u = min_ub_opt xs (if (comp_opt_le x u) then x else u)"
+
+fun dc_list_upper::"term duration_constraint list \<Rightarrow> int upper_bound option" where
+"dc_list_upper xs = map dc_to_ub xs |> (\<lambda>xs. min_ub_opt xs None)" 
+
+fun lower_spec::"ast_action_schema \<Rightarrow> _" where
+"lower_spec (Simple_Action_Schema n ps pre eff) = Some (lower_bound.GE 0)" | (* could also be None *)
+"lower_spec (Durative_Action_Schema n ps d cond eff) = (dc_list_lower d)"
+
+fun upper_spec::"ast_action_schema \<Rightarrow> _" where
+"upper_spec (Simple_Action_Schema n ps pre eff) = Some (upper_bound.LE 0)" | (* could also be None *)
+"upper_spec (Durative_Action_Schema n ps d cond eff) = (dc_list_upper d)"
+
+
 
 end
 
-locale ground_ast_problem = ast_problem P 
+locale ground_ast_problem_defs = ast_problem P
   for P :: ast_problem
 begin
 
-sublocale tp_nta_reduction_model_checking' 
-proof 
+text \<open>Begin: Taken from M. Vollath\<close>
+fun is_pos_lit :: "'a atom Formulas.formula \<Rightarrow> bool" where
+  f: "is_pos_lit \<bottom> = False" |
+  "is_pos_lit (\<^bold>\<not>\<bottom>) = True" |
+  "is_pos_lit (Atom (predAtm n args)) = True" |
+  "is_pos_lit (\<^bold>\<not>(Atom (predAtm n args))) = False" |
+  "is_pos_lit (Atom (eqAtm a b)) = False" |
+  "is_pos_lit (\<^bold>\<not>(Atom (eqAtm a b))) = False" |
+  "is_pos_lit _ = False"
 
+fun is_pos_conj :: "'a atom Formulas.formula \<Rightarrow> bool" where
+  "is_pos_conj (f \<^bold>\<and> g) \<longleftrightarrow> is_pos_lit f \<and> is_pos_conj g" |
+  "is_pos_conj f \<longleftrightarrow> is_pos_lit f"
+
+text \<open>End: Taken from M. Vollath\<close>
+
+fun pred_no_args::"predicate_decl \<Rightarrow> bool" where
+"pred_no_args (PredDecl p as) = (as = [])"
+
+fun act_no_args::"ast_action_schema \<Rightarrow> bool" where
+"act_no_args (Simple_Action_Schema n ps pre eff) = (ps = [])" |
+"act_no_args (Durative_Action_Schema n ps d pre eff) = (ps = [])" 
+
+fun act_pres_pos::"ast_action_schema \<Rightarrow> bool" where
+"act_no_args (Simple_Action_Schema n ps pre eff) = (is_pos_conj (map snd pre))" |
+"act_no_args (Durative_Action_Schema n ps d pre eff) = (is_pos_conj (map snd pre))" 
+
+lemma wf_pos_conj_fmla_imp_wf_atoms: 
+    assumes "wf_fmla M form"
+        and "is_pos_conj form"
+      shows "list_all (wf_fmla_atom M) (to_literals form)"
+  using assms
+  apply (induction form)
+  subgoal for x apply (cases x) by auto
+  subgoal by simp
+  subgoal for f 
+    apply (induction f)
+    subgoal for x apply (cases x) by auto
+    by auto
+  subgoal for f g
+    by (cases f) auto
+  by auto
+
+  
+qed
+
+end
+
+locale ground_ast_problem = 
+    ground_ast_problem_defs P +
+    wf_ast_problem P
+  for P :: ast_problem +
+  assumes positive_goal: "is_pos_conj (goal P)"
+      and preds_no_args: "list_all pred_no_args (predicates D)"
+      and acts_no_args: "list_all act_no_args (actions D)"
+      and positive_act_pres: "list_all (\<lambda>a. 
+      and no_functions: "functions D = []"
+begin
+  
+
+lemma wf_fmla_atom_in_props:
+  assumes "wf_fmla_atom M x"
+  shows "to_predicate x \<in> set props_spec"
+proof -
+  obtain p vs where
+    x: "x = Atom (predAtm p vs)"
+    "wf_pred_atom M (p, vs)"
+    using assms
+    apply (cases x)
+    subgoal for y 
+      apply (cases y) by auto
+    by auto
+  obtain Ts where
+    Ts: "sig p = Some Ts"
+    using x(2) unfolding wf_pred_atom.simps
+    apply (cases "sig p")
+    unfolding sig_def by auto
+  hence Ts_ran: "Ts \<in> ran sig" 
+    by (rule ranI)
+  hence p_dom: "p \<in> dom sig" using Ts by auto
+  have "snd ` set (map (\<lambda>x. case x of PredDecl p n \<Rightarrow> (p, n)) (predicates local.D)) = {[]}"
+  proof (rule equalityI)
+    show pred_args: "snd ` (set (map (\<lambda>x. case x of PredDecl p n \<Rightarrow> (p, n)) (predicates D))) \<subseteq> {[]}"
+    proof (intro  subsetI)
+      fix x
+      assume "x \<in> snd ` set (map (\<lambda>x. case x of PredDecl p n \<Rightarrow> (p, n)) (predicates local.D))" 
+      then obtain predd p' n' where
+        "predd \<in> set (predicates D)"
+        "predd = PredDecl p' n'"
+        "x = n'" 
+        unfolding set_map
+        unfolding image_image
+        apply -
+        apply (erule imageE)
+        subgoal for predd
+          apply (cases predd)
+          by auto
+        done
+      thus "x \<in> {[]}" using preds_no_args 
+        unfolding list_all_iff by fastforce
+    qed
+    show "{[]} \<subseteq> snd ` set (map (\<lambda>x. case x of PredDecl p n \<Rightarrow> (p, n)) (predicates local.D))"
+    proof -
+      have 1: "Ts \<in> snd ` set (map (\<lambda>x. case x of PredDecl p n \<Rightarrow> (p, n)) (predicates local.D))"
+        apply (rule set_mp)
+        apply (rule Misc.ran_map_of)
+        using Ts_ran
+        unfolding sig_def by auto
+      with pred_args
+      have "Ts = []" by blast
+      thus ?thesis using Ts_ran 1 by auto
+    qed
+  qed
+  have "fst ` set (map (\<lambda>x. case x of PredDecl p n \<Rightarrow> (p, n)) (predicates D)) = pred ` set (predicates D)"
+    apply (intro equalityI subsetI)
+    unfolding set_map image_image
+     apply (erule imageE)
+    subgoal for x predd
+      apply (cases predd)
+      using predicate_decl.sel by force
+    apply (erule imageE)
+    subgoal for x predd
+      apply (cases predd)
+      using predicate_decl.sel by force
+    done
+  then
+  show ?thesis
+    unfolding x to_predicate.simps
+    unfolding props_spec_def
+    using p_dom unfolding sig_def
+    unfolding dom_map_of_conv_image_fst by auto
+qed
+
+lemma start_snaps_wf:
+  assumes "a \<in> set actions_spec"
+  shows "wf_ground_action (at_start_spec a)"
+  using assms
+proof (induction a)
+  case (Simple_Action_Schema n ps pre eff)
+  show ?case 
+    unfolding at_start_spec.simps
+  proof (rule wf_inst_action_schema)
+    have 1: "ps = []" 
+      using acts_no_args Simple_Action_Schema
+      unfolding actions_spec_def list_all_iff by auto
+    show "action_params_match (Simple_Action_Schema n ps pre eff) []" 
+      unfolding action_params_match_def 1 by simp
+    show "wf_action_schema (Simple_Action_Schema n ps pre eff)"
+      using wf_domain unfolding wf_domain_def 
+      using Simple_Action_Schema unfolding actions_spec_def by blast
+  qed
+next
+  case (Durative_Action_Schema n ps d pre eff)
+  show ?case 
+    unfolding at_start_spec.simps
+  proof (rule wf_inst_durative_action_schema)
+    have 1: "ps = []" 
+      using acts_no_args Durative_Action_Schema
+      unfolding actions_spec_def list_all_iff by auto
+    show "action_params_match (Durative_Action_Schema n ps d pre eff) []"
+      unfolding action_params_match_def using 1 by simp
+    show "wf_action_schema (Durative_Action_Schema n ps d pre eff)"
+      using wf_domain unfolding wf_domain_def 
+      using Durative_Action_Schema unfolding actions_spec_def by blast
+  qed
+qed
+
+lemma end_snaps_wf:
+  assumes "a \<in> set actions_spec"
+  shows "wf_ground_action (at_end_spec a)"
+  using assms
+proof (induction a)
+  case (Simple_Action_Schema n ps pre eff)
+  show ?case 
+    unfolding at_end_spec.simps
+    unfolding non_ground_action_def by auto
+next
+  case (Durative_Action_Schema n ps d pre eff)
+  show ?case 
+    unfolding at_end_spec.simps
+  proof (rule wf_inst_durative_action_schema)
+    have 1: "ps = []" 
+      using acts_no_args Durative_Action_Schema
+      unfolding actions_spec_def list_all_iff by auto
+    show "action_params_match (Durative_Action_Schema n ps d pre eff) []"
+      unfolding action_params_match_def using 1 by simp
+    show "wf_action_schema (Durative_Action_Schema n ps d pre eff)"
+      using wf_domain unfolding wf_domain_def 
+      using Durative_Action_Schema unfolding actions_spec_def by blast
+  qed
+qed
+
+lemma over_all_snap_wf:
+  assumes "a \<in> set actions_spec"
+  shows "wf_ground_action (over_all_snap a)"
+  using assms
+proof (induction a)
+  case (Simple_Action_Schema n ps pre eff)
+  show ?case 
+    unfolding over_all_snap.simps
+    unfolding non_ground_action_def by auto
+next
+  case (Durative_Action_Schema n ps d pre eff)
+  show ?case 
+    unfolding over_all_snap.simps
+  proof (rule wf_inst_durative_action_schema)
+    have 1: "ps = []" 
+      using acts_no_args Durative_Action_Schema
+      unfolding actions_spec_def list_all_iff by auto
+    show "action_params_match (Durative_Action_Schema n ps d pre eff) []"
+      unfolding action_params_match_def using 1 by simp
+    show "wf_action_schema (Durative_Action_Schema n ps d pre eff)"
+      using wf_domain unfolding wf_domain_def 
+      using Durative_Action_Schema unfolding actions_spec_def by blast
+  qed
+qed
+
+lemma wf_ground_action_pres_in_props:
+  assumes "wf_ground_action h"
+  shows "(set \<circ> pre_spec) h \<subseteq> set props_spec"
+  using assms
+proof (induction h)
+  case (Ground_Action pre eff)
+  have 1: "list_all (wf_fmla_atom objT) (pre)"
+    using Ground_Action unfolding wf_ground_action.simps apply (induction eff)
+    using wf_effect.simps list_all_iff by auto
+  show ?case 
+    apply (rule subsetI)
+    unfolding comp_def pres_spec.simps
+    using 1 wf_fmla_atom_in_props 
+    unfolding list_all_iff by auto
+qed
+
+lemma wf_ground_action_adds_in_props:
+  assumes "wf_ground_action h"
+  shows "(set \<circ> adds_spec) h \<subseteq> set props_spec"
+  using assms
+proof (induction h)
+  case (Ground_Action pre eff)
+  have 1: "list_all (wf_fmla_atom objT) (adds eff)"
+    using Ground_Action unfolding wf_ground_action.simps apply (induction eff)
+    using wf_effect.simps list_all_iff by auto
+  show ?case 
+    apply (rule subsetI)
+    unfolding comp_def adds_spec.simps
+    using 1 wf_fmla_atom_in_props 
+    unfolding list_all_iff by auto
+qed
+
+lemma wf_ground_action_dels_in_props:
+  assumes "wf_ground_action h"
+  shows "(set \<circ> dels_spec) h \<subseteq> set props_spec"
+  using assms
+proof (induction h)
+  case (Ground_Action pre eff)
+  have 1: "list_all (wf_fmla_atom objT) (dels eff)"
+    using Ground_Action unfolding wf_ground_action.simps apply (induction eff)
+    using wf_effect.simps list_all_iff by auto
+  show ?case 
+    apply (rule subsetI)
+    unfolding comp_def dels_spec.simps
+    using 1 wf_fmla_atom_in_props 
+    unfolding list_all_iff by auto
+qed
+
+
+lemma init_in_props: "set init_spec \<subseteq> set props_spec"
+proof -
+  have 1: "\<forall>f\<in>set (init P). wf_fmla_atom objT f \<or> wf_func_assign f"
+    using wf_problem unfolding wf_problem_def wf_domain_def by auto
+  have "\<forall>f\<in>set (init P). wf_fmla_atom objT f" 
+  proof (intro strip ballI)
+    fix f
+    assume "f \<in> set (init P)"
+    then consider "wf_fmla_atom objT f" | "wf_func_assign f" using 1 by auto
+    thus "wf_fmla_atom objT f"
+    proof (cases)
+      case 1
+      then show ?thesis by simp
+    next
+      case 2
+      then obtain n as t where
+        f: "f = Atom (eqAtm (FuncEnt n as) (TimeEnt t))" 
+        apply (cases f)
+        subgoal for x
+          apply (cases x)
+           apply (simp)
+          subgoal for a b
+            apply (cases a; cases b)
+            by auto
+          done
+        by auto   
+      hence "wf_func_args objT (n,as)" using 2 by auto
+      hence False using no_functions func_sig_def by auto
+      thus ?thesis by auto
+    qed
+  qed
+  thus ?thesis using wf_fmla_atom_in_props init_spec_def by auto
+qed
+
+lemma goal_in_props: "set goal_spec \<subseteq> set props_spec"
+proof -
+  have "wf_fmla objT (goal P)"
+    using wf_problem unfolding wf_problem_def
+    unfolding props_spec_def goal_spec_def by auto
+  hence "list_all (wf_fmla_atom objT) (to_literals (goal P))" 
+    using wf_pos_conj_fmla_imp_wf_atoms positive_goal by auto
+  hence "set (map to_predicate (to_literals (goal P))) \<subseteq> set props_spec"
+    using wf_fmla_atom_in_props unfolding set_map list_all_iff by auto
+  thus ?thesis using goal_spec_def by auto
+qed
+
+sublocale tp_nta_reduction_model_checking' 
+  init_spec goal_spec at_start_spec at_end_spec 
+  over_all_spec 
+  lower_spec upper_spec 
+  pre_spec adds_spec dels_spec
+  0
+  props_spec actions_spec
+  act_to_name_spec prop_to_name_spec
+proof 
+  show "0 \<le> (0::int)" by auto
+  show "distinct props_spec"
+    using wf_problem
+    unfolding wf_problem_def wf_domain_def props_spec_def 
+    by simp
+  show "distinct actions_spec"
+  proof -
+    have "distinct (map ast_action_schema.name (actions local.D))"
+    using wf_problem
+    unfolding wf_problem_def wf_domain_def actions_spec_def 
+    by simp
+    hence "distinct (actions local.D)"
+      using distinct_map by blast
+    thus ?thesis unfolding actions_spec_def by auto
+  qed                                         
+  show "\<forall>a\<in>set actions_spec. distinct (over_all_spec a)"
+    apply (intro ballI)
+    subgoal for a
+      apply (induction a)
+       apply (subst over_all_spec.simps)
+       apply (subst over_all_snap.simps)
+       apply (subst non_ground_action_def)
+       apply simp
+      using distinct_remdups non_ground_action_def by simp
+    done
+  show "set goal_spec - set props_spec \<subseteq> set init_spec - set props_spec"
+    using init_in_props goal_in_props by auto
+  show "\<forall>a\<in>set actions_spec. action_and_prop_set.act_mod_props at_start_spec at_end_spec (set \<circ> adds_spec) (set \<circ> dels_spec) (set props_spec) a"
+  proof (rule ballI)
+    fix a
+    assume "a \<in> set actions_spec" 
+    thus "action_and_prop_set.act_mod_props at_start_spec at_end_spec (set \<circ> adds_spec) (set \<circ> dels_spec) (set props_spec) a"
+      by (intro action_and_prop_set.act_mod_propsI action_and_prop_set.snap_mod_propsI 
+          wf_ground_action_adds_in_props wf_ground_action_dels_in_props start_snaps_wf end_snaps_wf)
+  qed
+  show "action_set_and_props.action_consts at_start_spec at_end_spec (set \<circ> over_all_spec) (set \<circ> pre_spec) (set \<circ> adds_spec) (set \<circ> dels_spec) (set props_spec) (set actions_spec) \<subseteq> set init_spec - set props_spec"
+  proof (rule subsetI)
+    fix x
+    assume "x \<in> action_set_and_props.action_consts at_start_spec at_end_spec (set \<circ> over_all_spec) (set \<circ> pre_spec) (set \<circ> adds_spec) (set \<circ> dels_spec) (set props_spec) (set actions_spec)"
+    then obtain a where
+      a: "x \<in> action_and_prop_set.act_consts at_start_spec at_end_spec (set \<circ> over_all_spec) (set \<circ> pre_spec) (set \<circ> adds_spec) (set \<circ> dels_spec) (set props_spec) a" 
+      "a \<in> set actions_spec" unfolding action_set_and_props.action_consts_def by blast
+    then consider "x \<in> action_and_prop_set.snap_consts (set \<circ> pre_spec) (set \<circ> adds_spec) (set \<circ> dels_spec) (set props_spec) (at_start_spec a)"
+      | "x \<in> action_and_prop_set.snap_consts (set \<circ> pre_spec) (set \<circ> adds_spec) (set \<circ> dels_spec) (set props_spec) (at_end_spec a)"
+      | "x \<in> ((set \<circ> over_all_spec) a - set props_spec)" unfolding action_and_prop_set.act_consts_def by auto
+    hence "x \<in> {}" 
+    proof (cases)
+      case 1
+      hence "x \<in> undefined" unfolding action_and_prop_set.snap_consts_def
+      then show ?thesis sorry
+    next
+      case 2
+      then show ?thesis sorry
+    next
+      case 3
+      then show ?thesis sorry
+    qed
+        
+    show "x \<in> set init_spec - set props_spec" sorry
+  qed
 qed
 end
 end
