ROOT
@@ -1,26 +1,26 @@
 session Temporal_Planning_Base in Temporal_Planning_Base = Munta_Model_Checker +
-    sessions "List-Index"
-    theories
-      Base
-      ListMisc
-      Temporal_Plans 
-      Sequences
+  sessions "List-Index"
+  theories
+    Base
+    ListMisc
+    Temporal_Plans 
+    Sequences
 
 session TP_NTA_Reduction in TA_Network =
-    Temporal_Planning_Base + 
-    sessions Munta_Certificate_Checker
-    theories
-      NTA_Temp_Planning_Sem
-      TP_NTA_Reduction_Spec
-      TP_NTA_Reduction_Model_Checking
-      TP_NTA_Reduction_Correctness
+  Temporal_Planning_Base + 
+  sessions Munta_Certificate_Checker
+  theories
+    NTA_Temp_Planning_Sem
+    TP_NTA_Reduction_Spec
+    TP_NTA_Reduction_Model_Checking
+    TP_NTA_Reduction_Correctness
 
 session PDDL_TP_Reduction in Ground_PDDL_Exec_Imp = 
-    TP_NTA_Reduction +
-    sessions Temporal_AI_Planning_Languages_Semantics
-    theories 
-      PDDL_TP_Reduction 
-      Check_Unsolvability
-      Unsolvability_Code_Compile
+  TP_NTA_Reduction +
+  sessions Temporal_AI_Planning_Languages_Semantics
+  theories 
+    PDDL_TP_Reduction 
+    Check_Unsolvability
+    Unsolvability_Code_Compile
     
 
